gen-syntax/poplmark.v
@@ -1,4 +1,5 @@
-Require Import Subst Size util lib.
+Require Import Program.Equality ssreflect List.
+Require Import Subst Size util lib Decidable Ctxts.
 
 Inductive type : Type :=
 | TVar (x : var)
@@ -6,97 +7,146 @@ Inductive type : Type :=
 | Arr (A1 A2 : type)
 | All (A1 : type) (A2 : bind type).
 
-Definition ty_ctxt := list type.
-
 Instance subst_type : Subst type. gen_Subst. Defined.
-Instance substLemmas_type : SubstLemmas subst_type. 
+Instance substLemmas_type : SubstLemmas _ subst_type. 
 gen_SubstLemmas. Defined.
+Instance size_type : Size type. 
+assert(Size var). exact(fun _ => 0).
+gen_Size. Defined.
 
-Instance size_type : Size type. gen_Size. Defined.
-
-Inductive ty_get : ty_ctxt -> var -> type -> Prop :=
-| Get0 Delta A: ty_get (cons A Delta) 0 A.[ren(+1)]
-| GetS Delta x A B : ty_get Delta x B -> ty_get (cons A Delta) (S x) B.[ren(+1)]
-.
-
-Definition inj {A B : Type} (f : A -> B) := forall x y, f x = f y -> x = y. 
-
-Lemma ren_inj xi : inj xi -> inj (fun A => A.[ren xi]).
+Lemma ren_size_inv A : forall xi, size A.[ren xi] = size A.
 Proof.
-  unfold inj. intros H A B H'.
-  aind A; ssimpl in *.
-  - destruct B; arew.
-  - destruct B; arew.
-  - destruct B; ssimpl in H'; inversion H'. f_equal; arew.
-  - destruct B; ssimpl in H'; inversion H'. f_equal. arew. ssimpl in *.
-    eapply IHA0;[idtac|eassumption]. intros. destruct x; destruct y; arew.
+  induction A; intros; sizesimpl; repeat(ssimpl; try autorew); try somega.
 Qed.
 
-Lemma ty_get_weakening Delta A x B : ty_get Delta x A <-> ty_get (Delta,,B) (S x) A.[ren(+1)].
-Proof.
-  split.
-  - arew.
-  - intros. inversion H; subst. apply ren_inj in H4; arew.
-Qed.
+Fixpoint wf_ty Delta A := match A with
+  | TVar x => exists B, dep_get Delta x B
+  | Top => True
+  | Arr A B => wf_ty Delta A /\ wf_ty Delta B
+  | All A B => wf_ty Delta A /\ wf_ty Delta,,A B
+end.
 
-Inductive wf_ty Delta : type -> Prop :=
-| Wf_ty_TVar x B : ty_get Delta x B -> wf_ty Delta B -> wf_ty Delta (TVar x)
-| Wf_ty_Top : wf_ty Delta Top
-| Wf_ty_Arr A1 A2 : wf_ty Delta A1 -> wf_ty Delta A2 -> wf_ty Delta (Arr A1 A2)
-| Wf_ty_All A1 A2 : wf_ty Delta A1 -> wf_ty (Delta,, A1) A2 -> wf_ty Delta (All A1 A2)
-.
-(*
-Lemma wf_ty_weakening p Delta A B : p = (Delta, A) -> wf_ty Delta A -> wf_ty (Delta,,B) A.[ren(+1)].
-Proof.
-  
-Qed.*)
-
-Inductive sub (Delta : ty_ctxt) : type -> type -> Prop :=
+Inductive sub (Delta : list type) : type -> type -> Prop :=
 | SA_Top A : wf_ty Delta A -> sub Delta A Top
 | SA_Refl x : wf_ty Delta (TVar x) -> sub Delta (TVar x) (TVar x)
-| SA_Trans x A B : ty_get Delta x A -> sub Delta A B -> sub Delta (Var x) B 
+| SA_Trans x A B : dep_get Delta x A -> sub Delta A B -> sub Delta (Var x) B 
 | SA_Arrow A1 A2 B1 B2 : sub Delta B1 A1 -> sub Delta A2 B2 -> sub Delta (Arr A1 A2) (Arr B1 B2)
-| SA_All A1 A2 B1 B2 : sub Delta B1 A1 -> sub (cons B1 Delta) A2 B2 -> sub Delta (All A1 A2) (All B1 B2)
+| SA_All A1 A2 B1 B2 : sub Delta B1 A1 -> wf_ty Delta B1 -> sub (Delta,,B1) A2 B2 -> sub Delta (All A1 A2) (All B1 B2)
 .
 
-Require Import util lib Program.Equality.
-
-Lemma wf_ren Delta1 Delta2 A xi zeta : wf_ty Delta1 A.[ren zeta] -> (forall x B, ty_get Delta1 (zeta x) B.[ren zeta] -> ty_get Delta2 (xi x) B.[ren xi]) -> wf_ty Delta2 A.[ren xi].
+Lemma wf_weak Delta1 Delta2 A xi : 
+  wf_ty Delta1 A -> 
+  (forall x B, dep_get Delta1  x B -> exists B', dep_get Delta2 (xi x) B') -> 
+  wf_ty Delta2 A.[ren xi].
 Proof.
-  intros H. daind H. destruct A.
-eapply IHwf_ty. eassumption.
-  ssimpl. constructor. arew. apply IHwf_ty2. intros. destruct x; ssimpl in *. 
-  - inversion H2; subst. ssimpl. pose proof (Get0 Delta2 A1.[ren xi]). ssimpl in H3. apply H3. 
-  - inversion H2; subst. ssimpl in *. pose proof (GetS Delta2 (xi x) A1.[ren xi] B0.[ren xi]). ssimpl in H3. apply H3. arew.
+  intros H. aind A. ssimpl.
+  eapply IHA0. eassumption. intros.
+  destruct x; ssimpl; arew; ssimpl. unfold lift. simpl. 
+  edestruct H0; arew.
 Qed.
 
-Lemma sub_wf Delta A B : sub Delta A B -> wf_ty Delta A /\ wf_ty Delta B.
+Corollary wf_weak' Delta1 Delta2 A : 
+  wf_ty Delta1 A -> 
+  (length Delta1 <= length Delta2) -> 
+  wf_ty Delta2 A.
 Proof.
-  intros H. 
-  induction H; auto; arew.
-  constructor. intuition. 
-  autorevert A2. induction A2; intros; arew.
-  - destruct x.
-    + econstructor. constructor. eapply wf_ren. eassumption. intros. apply ty_get_weakening. assumption.
-    + inversion H7; subst. econstructor. apply ty_get_weakening.  eapply ty_get_weakening. eassumption. eapply wf_ren. eapply wf_ren.
-
-eassumption. intros. ssimpl. inversion H1; subst. econstructor.
-  - 
-  constructor.
-  - arew. destruct v; arew. 
-  - arew. eapply IHA2_1; arew.
+  intros. 
+  cutrewrite(A = A.[ren id]);[idtac|now ssimpl]. 
+  eapply wf_weak; eauto.
+  intros.
+  apply dep_get_defined.
+  cut(id x < length Delta1). omega.
+  apply dep_get_defined.
+  eexists. eassumption.
 Qed.
 
-
-Lemma sub_refl Delta A : sub Delta A A.
+Lemma sub_refl Delta A : wf_ty Delta A -> sub Delta A A.
 Proof.
-  revert Delta. induction A; eauto using sub.
+  revert Delta. induction A; simpl; intuition; eauto using sub.
 Qed.
 
-Ltac inv H := inversion H; subst; clear H.
-Lemma sub_trans Delta A B C: sub Delta A B -> sub Delta B C -> sub Delta A C.
+Lemma sub_weak Delta1 Delta2 A1 A2 xi : sub Delta1 A1 A2 -> 
+  (forall x B, dep_get Delta1 x B -> dep_get Delta2 (xi x) B.[ren xi]) -> 
+  sub Delta2 A1.[ren xi] A2.[ren xi] .
 Proof.
-  revert Delta A C. induction B.
-  - intros. inv H. assumption.
-    econstructor 3. eassumption.
+   intros H. aind H.
+   - constructor. eapply wf_weak; now eauto.
+   - econstructor; ssimpl.
+     + now eauto.
+     + eapply wf_weak; now eauto.
+     + apply IHsub2. intros.
+       destruct x; ssimpl; arew; ssimpl; rewrite (ren_uncomp _ _ (+1)); arew. 
+Qed.
+
+Lemma sub_wf {Delta A B} : sub Delta A B -> wf_ty Delta A /\ wf_ty Delta B.
+Proof.
+  intros H. aind H.
+  eapply wf_weak'. eassumption.
+  now simpl.
+Qed.
+
+Lemma sub_trans' n : 
+  (forall Delta A B C, n = size B -> sub Delta A B -> sub Delta B C -> sub Delta A C) /\
+  (forall Delta' Delta  B B' A C, n = size B -> sub Delta,,B,,,Delta' A C -> sub Delta B' B -> sub Delta,,B',,,Delta' A C)
+.
+Proof.
+  induction n as [n IH] using (size_rec (fun x => x)).
+  apply conj'.
+  {
+    intros Delta A B C ? H_AB H_BC. subst.
+    revert C H_BC.
+    induction H_AB; prepare.
+    - now arew.
+    - econstructor; now prepare.
+    - inv H_BC. 
+      + constructor. simpl. intuition. now eapply (sub_wf H_AB1). now eapply (sub_wf H_AB2).
+      + constructor; eapply IH; eauto; somega.
+    - inv H_BC.
+      + constructor; constructor. 
+        * eapply sub_wf; now eauto. 
+        * eapply wf_weak'. now eapply (sub_wf H_AB2). now simpl.
+      + rename B0 into C1. rename B3 into C2.
+        constructor; eauto.
+        * eapply IH; eauto; somega.
+        * eapply IH; eauto; try somega.
+          refine (proj2 (IH _ _) nil _ _ _ _ _ _ _ _); eauto; somega.
+  }
+  {
+    intros H_trans Delta' Delta B B' A C ? H H_B'B. subst.
+    revert B' H_B'B.
+    depind H; prepare.
+    - constructor.
+      eapply wf_weak'. eassumption.
+      repeat rewrite app_length. simpl. omega.
+    - constructor. simpl.
+      apply dep_get_defined. apply dep_get_defined in H.
+      repeat rewrite -> app_length in *. simpl in *. omega.
+    - decide (x = length Delta').
+      + subst.
+        econstructor. { apply dep_get_repl. }
+        apply dep_get_steps' with (x := 0) in H.
+        destruct H as [? [? H]]. inv H.
+        eapply H_trans;[idtac | eapply sub_weak; try eassumption | idtac].
+        * now rewrite ren_size_inv.
+        * intros. change Delta,,B' with Delta,,,(nil,,B'). rewrite app_assoc.
+          cutrewrite (S (length Delta') = length (nil,,B',,,Delta')); 
+            first by apply dep_get_steps.
+          rewrite app_length. simpl. omega.
+        * ssimpl in IHsub.
+          eapply IHsub; now eauto. 
+      + econstructor; eauto.
+        eapply dep_get_repl; now eauto.
+    - constructor; now eauto.
+    - constructor. 
+      + now eauto. 
+      + eapply wf_weak'. eassumption.
+        repeat rewrite app_length. simpl. omega.
+      + change Delta,,B',,,Delta',,B1 with Delta,,B',,,(Delta',,B1).
+        eapply IHsub2; eauto. reflexivity.
+  }
+Qed.
+
+Corollary sub_trans Delta A B C: sub Delta A B -> sub Delta B C -> sub Delta A C.
+Proof.
+  intros. eapply sub_trans'; eauto.
 Qed.
