gen-syntax/Decidable.v
@@ -1,0 +1,9 @@
+Definition dec (X : Prop) : Type := {X} + {~ X}.
+Class Dec (X : Prop) : Type := decide : dec X.
+Arguments decide X {_}.
+
+Ltac gen_Dec := unfold Dec; unfold dec; decide equality.
+
+Instance decide_eq_nat (x y : nat) : Dec (x = y). gen_Dec. Defined.
+
+Tactic Notation "decide" constr(p) := destruct (decide p).
